WIP on concurrent hash maps

Test/uncooperativeconcurrency/concurrenthashmap.dfy
@@ -6,27 +6,40 @@ class Entry<K(==), V> {
   ghost const Repr: set<object>
 
   constructor(hash: int, key: K, value: V, next: Entry?<K, V>)
-    ensures next == null || this !in next.Repr;
+    ensures next == null || this !in next.Repr
+    ensures this.next == next && this.key == key && this.value == value
+    ensures this.Repr == if next == null then {this} else {this} + next.Repr
     {
       this.hash := hash;
       this.key := key;
       this.value := value;
+      this.next := next;
       this.Repr := if next == null then {this} else {this} + next.Repr;
     }
 
+  function Count(): (res: nat)
+    reads this, Repr
+    decreases |Repr|
+    requires Invariant()
+  {
+    1 + (if next == null then 0 else next.Count())
+  }
+
   ghost predicate Invariant()
     reads this, Repr
+    decreases |Repr|
   {
     && this in Repr
     && if this.next == null then true
        else
-         && next.Repr == {this} + Repr
+         && Repr == {this} + next.Repr
          && this !in next.Repr
+         && next in Repr
          && next.Invariant()
   }
 
   // Ensures that the first entries override the last ones
-  function ToModel(): map<K, V> reads this, Repr
+  ghost function ToModel(): map<K, V> reads this, Repr
     requires Invariant()
     decreases |Repr|
   {
@@ -35,11 +48,20 @@ class Entry<K(==), V> {
   }
 }
 
+class Segment {
+  var count: int
+  constructor() {
+      this.count := 0;
+    }
+}
+
 class ConcurrentHashMap<K(==), V> {
   var entries: array<Entry?<K, V>>
+  var segments: array<Segment>
+
   ghost var model: map<K, V>
   ghost var Repr: set<object>
-  function {:vcs_split_on_every_assert} {:rlimit 1000} ToModel(startIndex: nat): map<K, V> reads this
+  ghost function {:vcs_split_on_every_assert} {:rlimit 1000} ToModel(startIndex: nat): map<K, V> reads this
     reads this, Repr
     requires startIndex <= entries.Length
     requires Invariant()
@@ -50,15 +72,100 @@ class ConcurrentHashMap<K(==), V> {
     var entry := entries[startIndex];
     rec + (if entry == null then map[] else entries[startIndex].ToModel())
   }
+  ghost predicate InvariantPerEntry2(i: int)
+    reads this, entries, segments, Repr
+    requires entries.Length == segments.Length
+    requires 0 <= i < segments.Length
+    requires InvariantPerEntry(entries[i])
+  {
+    segments[i] in Repr &&
+    if entries[i] != null then
+      && segments !in entries[i].Repr
+      && segments[i].count == entries[i].Count()
+    else
+      && segments[i].count == 0
+  }
+  ghost predicate InvariantPerEntry(entry: Entry?<K, V>)
+    reads this
+    reads entry
+    reads if entry != null then entry.Repr else {}
+  {
+    entry != null ==>
+      && this !in entry.Repr
+      && entries !in entry.Repr
+      && entry in Repr
+      && entry.Repr <= Repr
+      && entry.Invariant()
+  }
   ghost predicate Invariant()
     reads this, Repr
   {
     && this in Repr
     && entries in Repr
+    && segments in Repr
+    && entries.Length == segments.Length
+    && entries.Length >= 1
     && (forall i: nat | 0 <= i < this.entries.Length ::
-          entries[i] != null ==>
-            && entries[i] in Repr
-            && entries[i].Repr <= Repr
-            && entries[i].Invariant())
+          (entries[i] != null ==> entries[i] in Repr && entries[i].Repr <= Repr) &&
+          InvariantPerEntry(entries[i]) && InvariantPerEntry2(i))
+    && (forall i: nat, j: nat | i < entries.Length && j < entries.Length && i != j ::
+          entries[i] == null || entries[j] == null ||
+          entries[i].Repr !! entries[j].Repr)
   }
+
+  function Hash(k: K): int // Needs to be given!
+
+  method /*{:only}*/ {:vcs_split_on_every_assert} {:rlimit 3000} Put(k: K, v: V) returns (oldValueIfExisted: V)
+    requires Invariant()
+    modifies Repr
+    ensures Invariant()
+    {
+      var hash := Hash(k);
+      var indexEntry := hash % entries.Length;
+      var e := entries[indexEntry];
+      assert InvariantPerEntry(entries[indexEntry]);
+      assert e != null ==> e in Repr;
+      while(e != null)
+        invariant Invariant()
+        invariant e != null ==> e in Repr && e.Invariant() && e.Repr <= Repr
+        decreases if e == null then 0 else e.Count()
+      {
+        if e.hash == hash && k == e.key { // if key already exist means updating the value
+          var oldValue := e.value;
+          assert Invariant();
+          e.value := v;
+          assert Invariant();
+          return oldValue;
+        }
+        e := e.next;
+      }
+      ghost var oldHead := entries[indexEntry];
+      var newEntry := new Entry(hash, k, v, entries[indexEntry]);
+      assert newEntry !in Repr;
+      Repr := {newEntry} + Repr;
+      assert newEntry.next != null ==> newEntry.next.Invariant();
+      assert /*{:only} */&& newEntry in Repr
+                     && newEntry.Repr <= Repr
+                     && newEntry.Invariant();
+      assert this as object != entries as object;
+      assert this as object != segments as object;
+      entries[indexEntry] := newEntry;
+      segments[indexEntry].count := segments[indexEntry].count + 1;
+      assert {:only} Invariant() by {
+        assert forall i: nat | 0 <= i < this.entries.Length ::
+            InvariantPerEntry(entries[i]) by {
+          forall i: nat | 0 <= i < this.entries.Length ensures
+              InvariantPerEntry(entries[i]) {
+            if i == indexEntry {
+              assert InvariantPerEntry(entries[i]);
+            } else {
+              assert{:only} InvariantPerEntry(entries[i]) by {
+
+              }
+            }
+          }
+        }
+      }
+      return v;
+    }
 }
